variable history v1

theories/variable.v
@@ -5,36 +5,61 @@ From iris.program_logic Require Export atomic.
 From iris.heap_lang Require Import proofmode notation par.
 
 Class histG Σ := HistG {
-  hist_inG :> inG Σ (frac_authR (gmapUR positive (exclR valO)))
+  hist_inG :> inG Σ (frac_authR (gmapUR mnat (exclR valO)));
+  timestamp_inG :> inG Σ (exclR mnatR)
 }.
 Definition histΣ : gFunctors :=
-  #[GFunctor (frac_authR (gmapUR positive (exclR valO)))].
+  #[GFunctor (frac_authR (gmapUR mnat (exclR valO))); GFunctor (exclR mnatR)].
 Instance subG_histΣ {Σ} : subG histΣ Σ → histG Σ.
 Proof. solve_inG. Qed.
 
-Section asdf.
+Section var.
   Context `{!heapG Σ} `{histG Σ} (N : namespace).
 
   Definition new : val := λ: "v", ref "v".
   Definition set : val := λ: "l" "x", "l" <- "x".
 
-  Definition is_hist l γ := inv N ((l ↦ -) ∗ (∃ hs, own γ (●F hs))).
+  Definition last_op (t : mnat) v (hs : gmapUR mnat (exclR valO)) : iProp Σ :=
+    ⌜(∀ (t' : mnat), (t' ∈ (dom (gset mnat) hs) → t' ≤ t))
+    ∧ hs !! t = Some (Excl v) ⌝.
 
-  Lemma set_spec (l : loc) (γ : gname) (q : Qp) (v : val) :
-    is_hist l γ -∗
-    <<< ∀ hs, own γ (◯F{q} hs) >>>
+  Definition is_hist l γh γt :=
+    inv N (∃ v, (l ↦ v) ∗
+                (∃ hs (t : mnat),
+                    own γh (●F hs) ∗
+                    own γt (Excl t) ∗
+                    last_op t v hs)).
+
+  Lemma set_spec (l : loc) (γh γt : gname) (q : Qp) (v : val) :
+    is_hist l γh γt -∗
+    <<< ∀ hs, own γh (◯F{q} hs) >>>
       set #l v @ ⊤ ∖ ↑N
-    <<< ∃ (t:positive),
-        own γ (◯F{q} (hs ⋅ {[t:=Excl v]})),
+    <<< ∃ (t : mnat),
+        own γh (◯F{q} (<[t :=Excl v]> hs)),
         RET #() >>>.
   Proof.
     iIntros "#Hist" (Φ) "AU". wp_lam; wp_let.
-    iInv N as ">[Hl H●]".
-    iDestruct "Hl" as (?) "Hl". iDestruct "H●" as (hsM) "H●".
+    iInv N as (v') ">[Hl H]".
+    iDestruct "H" as (hsM tM) "[H● [Ht [% _]]]". rename H0 into tM_max.
     iMod "AU" as (hs) "[H◯ [_ Hclose]]".
-    wp_store.
-    iMod ("Hclose" with "[H◯]") as "$". iModIntro; iModIntro; iNext.
-    iSplitL "Hl"; eauto.
-End asdf.
-
-(* history of variable value *)
+    iMod (own_update with "Ht") as "Ht";
+      first by apply (cmra_update_exclusive (Excl (S tM))).
+    iMod (own_update_2 with "H● H◯") as "[H● H◯]".
+    { apply frac_auth_update, (alloc_local_update _ _ (S tM) (Excl v)); last done.
+      rewrite <-(not_elem_of_dom (D:=gset mnat)).
+      intro. apply tM_max in H0. lia. }
+    wp_store. clear v'.
+    iMod ("Hclose" with "[H◯]") as "$"; first done.
+    iModIntro; iModIntro; iNext.
+    iExists v. iSplitL "Hl"; first done.
+    iExists (<[S tM:=Excl v]> hsM), (S tM). iFrame.
+    iPureIntro. split; last by rewrite lookup_insert.
+    intros t'.
+    rewrite (dom_insert (M:=gmap mnat) (D:=gset mnat) (A:=excl valO)).
+    rewrite elem_of_union elem_of_singleton.
+    intro Ht'.
+    destruct Ht' as [Ht'|Ht'].
+    - by rewrite Ht'.
+    - apply tM_max in Ht'. lia.
+  Qed.
+End var.
